\documentclass{report}

\usepackage{a4}

\usepackage[english]{babel}
\usepackage[utf8]{inputenc}
\usepackage{amsmath, amssymb, mathtools, esint, bbold}
\usepackage{graphicx}
\usepackage{color}
\usepackage{datetime}
\usepackage[hidelinks]{hyperref}
\usepackage{enumitem}
\usepackage{stmaryrd}

\setlength{\parindent}{0em} 

\usepackage{amsthm}
\newtheoremstyle{tommy}% ⟨name ⟩
{15pt}% ⟨Space above ⟩1
{15pt}% ⟨Space below ⟩1
{\normalfont}% ⟨Body font ⟩
{}% ⟨Indent amount ⟩2
{\bfseries}% ⟨Theorem head font⟩
{}% ⟨Punctuation after theorem head ⟩
{0.7em}% ⟨Space after theorem head ⟩3
{}% ⟨Theorem head spec (can be left empty, meaning ‘normal’)⟩

\theoremstyle{tommy}
\newtheorem{defn}{Definition}
\newtheorem{thm}[defn]{Theorem}
\newtheorem{lem}[defn]{Lemma}
\newtheorem{nota}[defn]{Notation}
\newtheorem{cor}[defn]{Corrolary}
\newtheorem{prop}[defn]{Proposition}
\newtheorem{eg}[defn]{Example}
\newtheorem{rem}[defn]{Remark}
\newtheorem{ex}[defn]{Exercise}

% Counter
\usepackage{chngcntr}
\counterwithin{defn}{chapter}

\renewcommand\div{\operatorname{div}}
\renewcommand\qedsymbol{\(\blacksquare\)}

\title{Partial Differerential Equations \\ Thành Nam Phan \\ Winter Semester 2021/2022}
\author{Lecture notes \TeX{}ed by Thomas Eingartner}
\date{\today, \currenttime}

\begin{document}

\maketitle
\tableofcontents
\newpage



\chapter{Introduction}

A differential equation is an equation of a function and its derivatives. 

\begin{eg} (Linear ODE)
  Let \(f: \mathbb{R} \to \mathbb{R}\),
  \begin{align*}
    \begin{cases}
      f(t) = a f(t) \text{ for all } t \ge 0, a \in \mathbb{R} \\
      f(0) = a_0
    \end{cases}
  \end{align*}
  is a linear ODE (Ordinary differential equation). The solution is: \(f(t) = a_0 e^{at}\) for all \(t \ge 0\).
\end{eg}

\begin{eg} (Non-Linear ODE) \(f: \mathbb{R} \to \mathbb{R}\)
  \begin{align*}
    \begin{cases}
      f'(t) = 1 + f^2(t) \\
      f(0) = 1
    \end{cases}
  \end{align*}
  Lets consider \(f(t) = \tan(t) = \frac{\sin(t)}{\cos(t)}\). Then we have \[f'(t) = \frac{1}{\cos(t)} = 1 + \tan^2(t) = 1 + f^2(t),\] but this solution only is \emph{good} in \((- \pi, \pi)\). It's a problem to extend this to \(\mathbb{R} \to \mathbb{R}\).
\end{eg}

A PDE (Partial Differential Equation) is an equation of a function of 2 or more variables and its derivatives.

\begin{rem}
  Recall for \( \Omega \subseteq \mathbb{R}^d\) open and \(f: \Omega \to \{\mathbb{R}, \mathbb{C}\}\) the notation of partial derivatives:
  \begin{itemize}
    \item \(\partial_{x_i} f(x) = \lim_{h \to 0} \frac{f(x + he_i) - f(x)}{h}, \text{where } e_i = (0, 0, \dots, 1, \dots, 0, 0) \in \mathbb{R}^d\)
    \item \(D^\alpha f(x) = \partial_{x_1}^{\alpha_1} \cdots \partial_{x_d}^{\alpha_d} f(x), \text{where } \alpha \in \mathbb{N}^d\)
    \item \(Df = \nabla f = (\partial{x_1}, \ldots, \partial_{x_d})\)
    \item \(\Delta f = \partial_{x_1}^2 + \cdots + \partial^2_{x_d} f\)
    \item \(D^k f = (D^\alpha f)_{|\alpha| = k},  \text{where } |\alpha| = \sum_{i=1}^d |\alpha_i|\)
    \item \(D^2 f = (\partial_{x_i} \partial_{x_j} f)_{1 \le i, j \le d}\)
  \end{itemize}
\end{rem}

\begin{defn}
  Given a function \( F \). Then the equation of the form 
  \begin{align*}
    F(D^k u(x), D^{k-1} u(x), \dots, Du(x), u(x), x) = 0 
  \end{align*}
  with the unknown function \(u:\ \Omega \subseteq \mathbb{R}^d \longrightarrow \mathbb{R}\) is called a \emph{PDE of order \(k\)}.
  \begin{itemize}
    \item Equations \(\sum_d a_\alpha(x) D^\alpha u(x) = 0\), where \(a_\alpha\) and \(u\) are unknown functions are called \emph{Linear PDEs}. 
    \item Equations \(\sum_{|\alpha| = k} a_\alpha(x) D^\alpha u(x) + F(D^{k-1}u, D^{k-2}u, \dots, Du, u, x) = 0\) are called \emph{semi-linear PDEs}.
  \end{itemize}
\end{defn}

Goals: For \emph{solving a PDE} we want to
\begin{itemize}
  \item Find an explizit solution! This is in many cases impossible.
  \item Prove a \emph{well-posted theory} (existence of solutions, uniqueness of solutions, continuous dependence of solutions on the data)
\end{itemize}

We have two notations of solutions:
\begin{enumerate}
  \item Classical solution: The solution is continuous differentiable (e.g. \( \Delta u = f  \leadsto u \in C^2  \))
  \item Weak Solutions: The solution is not smooth/continuous
\end{enumerate}

\begin{defn} (Spaces of continous and differentiable functions)
  Let \(\Omega \subseteq R^d\) be open
  \begin{align*}
    C(\Omega) &= \left\{ f: \ \Omega \to \mathbb{R} \mid f \text{ continuous} \right\} \\
    C^k(\Omega) &= \left\{ f: \ \Omega \to \mathbb{R} \mid D^\alpha f \text{ is continuous for all } |\alpha| \le k \right\}
  \end{align*}
\end{defn}

Classical solution of a PDE of order \(k \leadsto C^k\) solutions!
\begin{align*}
  L^p(\Omega) = \left\{ f: \ \Omega \to \mathbb{R} \text{ lebesgue measurable} \mid \int_\Omega |f|^p d\lambda < \infty, 1 \le p < \infty \right\}
\end{align*}

Sobolev Space:
\begin{align*}
  W^{k,p}(\Omega)= \left \{ f \in L^p(\Omega) \mid \forall \alpha \in \mathbb{N}^n \text{ with } |\alpha| \leq k: D^{\alpha}f \in L^p(\Omega) \text{exists}  \right \}
\end{align*}

In this course we will investigate
\begin{itemize}
  \item Laplace / Poisson Equation: \(-\Delta u = f\)
  \item Heat Equation: \(\partial_t u - \Delta u = f\)
  \item Wave Equation: \(\partial_t^2 - \Delta u = f\)
  \item Schrödinger Equation: \(i \partial_t u - \Delta u = f\)
\end{itemize}


\chapter{Laplace / Poisson Equation}

\section{Laplace Equation}
\(- \Delta u = 0\) (Laplace) or \(-\Delta u = f(x)\) (Poisson).

\begin{defn} (Harmonic Function)
  Let \(\Omega\) be an open set in \(\mathbb{R}^d\). If \(u \in C^2(\Omega)\) and \(\Delta u = 0\) in \(\Omega\), then \(u\) is a harmonic function in \(\Omega\).
\end{defn}

\begin{thm} (Gauss-Green Theorem)\label{gauss-green}
  Let \(A \subseteq \mathbb{R}^d\) open, \(\vec{F} \in C^1(A, \mathbb{R}^d)\) and \(K \subseteq A\) compact with \(C^1\) boundary. Then
  \[ \int_{\partial K} \vec{F} \cdot \vec{\nu}\ dS(x) = \int_K \div(\vec{F})\ dx \]
  where \(\nu\) is the outward unit normal vector field on \(\partial K\).
Thus
\begin{align*}
  \int_{\partial V} \nabla u \cdot \vec{\nu}\ dS(x)
  = \int_V \div(\nabla u) \ dx
  = \int_V \Delta u(x) \ dx
\end{align*}
for any \(V \subseteq \Omega \) open.
\end{thm}


\begin{thm}(Green's Identities)\label{green-identities}
  Let \(A \subseteq \mathbb{R}^d\) open, \(K \subseteq A\) d-dim. compactum with \(C^1\) boundary and \(f, g \in C^2(A)\)
  \begin{enumerate}
    \item Green's first identity (Partial Integration): \begin{align*}
      \int_K \nabla f \cdot \nabla g \, dx = \int_{\partial K} f \frac{\partial g}{\partial \nu} \, dS - \int_K f \Delta g \, dx
    \end{align*}
    where \(\frac{\partial g}{\partial \nu} = \partial_\nu g = \nu \cdot \nabla g\)
    \item Green's second identity: \begin{align*}
      \int_K f \Delta g - (\Delta f) g \, dx = \int_{\partial K} \left(f \frac{\partial g}{\partial \nu} - g \frac{\partial f}{\partial \nu}\right) \, dS
    \end{align*}
  \end{enumerate}
\end{thm}

\begin{ex}
  Let \(\Omega \subseteq \mathbb{R}^d\) open, let \(f: \Omega \to \mathbb{R}\) be continuous. Prove that if \( \int_B f(x) \ dx = 0 \), then \( u \equiv 0 \) in \(\Omega\).
\end{ex}

\begin{thm} (Fundamential Lemma of Calculus of Variations)
  Let \(\Omega \subseteq \mathbb{R}^d\) open, let \(f \in L^1(\Omega)\). If 
  \(\int_B f(x) \ dx = 0\) for all \(x \in B_r(x) \subseteq \Omega\), then \(f(x) = 0\) a.e. (almost everywhere) \(x \in \Omega\).
\end{thm}

\begin{rem} (Solving Laplace Equation)
  \(-\Delta u = 0\) in \(\mathbb{R}^d\). Consider the case when \(u\) is radial, i.e. \(u(x) = v(|x|)\), \(v: \mathbb{R} \to \mathbb{R}\). Denote \(r = |x|\), then 
  \[
    \frac{\partial r}{\partial x} 
    = \frac{\partial}{\partial x_i}  \left(\sqrt{x_1^2 + \dots + x_d^2}\right) \\
    = \frac{2 x_i}{2{\sqrt{x_1^2 + \dots + x_d^2}}} \\
    = \frac{x_i}{r}
  \]
  Then
  \begin{align*}
    \partial_{x_i} u &= \partial_{x_i} v = (\partial_r v) \frac{\partial r}{\partial {x_i}} 
    = v'(r) \frac{x_i}{r} \\
    \partial^2_{x_i} u 
    &= \partial_{x_i} \left(v(r)' \frac{x_i}{r}\right) 
    = (\partial_{x_i}v(r)') \frac{x_i}{r} + v'(r) \partial_{x_i} \left(\frac{x_i}{r}\right) \\
    &= (\partial_r v'(r))\left(\frac{dr}{\partial_{x_i}}\right) \frac{x_i}{r} + v'(r)\left( \frac{1}{r} - \frac{x_i}{r^2}(\partial_{x_i} r) \right) 
    = v'(r) \frac{x_i^2}{r^2} + v'r(r)\left(\frac{1}{r} - \frac{x_i^2}{r^3}\right)
  \end{align*}

  So we have \(\Delta u = \left( \sum_{i=1}^d d_{x_i}^2 \right) u = v''(r) + v'(r) (\frac{d}{r} - \frac{1}{r})\)

  Thus \(\Delta u = v'(r) + v(r) \frac{d-1}{r}\). We consider \(d \ge 2\). Laplace operator \(\Delta u = 0\) now becomes \(v''(r) + v'(r) \frac{d-1}{r} = 0\) \\
  \(\Rightarrow\) \(\log(v(r))' = \frac{v'(r)}{v(r)} = - \frac{d-1}{r} = -(d-1)(\log r)'\) (recall \(log(f)' = \frac{f'}{f}\)) \\
  \(\Rightarrow v'(r) = \frac{1}{v^{d-2} + \text{ const.}}\) \\
  \(\begin{cases}
    \frac{const}{r^{d-2}} + const xx + const &,d \ge 3 \\
    const \log(r) + const xx r + const &,d = 2
  \end{cases}\)
\end{rem}

\begin{defn} 
  (Fundamential Solution of Laplace Equation)
  \begin{align*}
    \Phi(x) = \begin{cases}
      - \frac{1}{2 \pi} \log(|x|), & d = 2 \\
      \frac{1}{(d-2) d |B_1|} \frac{1}{|x|^{d-2}}, & d \ge 3
    \end{cases}
  \end{align*}
  
  Where \( |B_1| \) is the Volume of the ball \(B_1(0) = B(0, 1) \subseteq \mathbb{R}^d\).

\end{defn}

\begin{rem}
  \(\Delta \Phi(x) = 0\) for all \(x \in \mathbb{R}^d\) and \(x \ne 0\). 
\end{rem}


\section{Poisson-Equation}
The Poisson-Equation is \(-\Delta u(x) = f(x)\) in \(\mathbb{R}^d\). The explicit solution is given by
\begin{align*}
  u(x) &= (\Phi \star f)(x)
  = \int_{\mathbb{R}^d} \Phi(x-y)f(y) \ dy 
  = \int_{\mathbb{R}^d} \Phi(y)f(x-y) \ dy
\end{align*}
This can be heuristically justifyfied with \[-\Delta (\Phi \star f) = (-\Delta \Phi) \star f = \delta_0 \star f = f\]


\begin{thm}
  Assume \(f \in C_c^2(\mathbb{R}^d)\). Then \(u = \Phi \star f\) satisfies that \(u \in C^2(\mathbb{R}^d)\) and \(- \Delta u(x) = f(x)\) for all \(x \in \mathbb{R}^d\)
\end{thm}


\begin{proof}
  By definition we have
  \begin{align*}
    u(x) &= \int_{\mathbb{R}^d} \Phi(y) f(x-y) \, dy.
  \end{align*}
  First we check that \(u\) is continuous: Take \(x_k \to x_0\) in \(\mathbb{R}^d\). We prove that \(u(x_n) \xrightarrow{n} u_0\), i.e.
  \begin{align*}
    \lim_{n \to \infty} \int_{\mathbb{R}^d} \Phi(y) f(x_n - y) \ dy = \int_{\mathbb{R}^d} \Phi(y) f(x_0 - y) \ dy
  \end{align*}
  This follows from the Dominated Convergence Theorem. More precisely:
  \begin{align*}
    \lim_{n \to \infty} \Phi(y) f(x_n -y) = \Phi(y) f(x_0 - y) \quad \text{ for all } y \in \mathbb{R}^d \setminus \{0\}
  \end{align*}
  and 
  \begin{align*}
    |\Phi(y) f(x-y)| &\le \| f ||_{L^\infty} \cdot \mathbb{1}(|y| \le R) \cdot |\Phi(y)| \in L^1(\mathbb{R}^d, dy)
  \end{align*}
  where \(R > 0\) depends on \(\{x_n\}\) and \(\operatorname{supp}(f)\) but independent of \(y\). Now we compute the derivatives:
  \begin{align*}
    \partial_{x_i} u(x) 
    &= \partial_{x_i} \int_{\mathbb{R}^d} \Phi(y) f(x-y) \ dy
    = \lim_{h \to 0} \int_{\mathbb{R}^d} \Phi(y) \frac{f(x + h e_i - y) - f(x-y)}{h} \ dy \\
    \text{(dom. conv.)} \quad &= \int \Phi(y) \partial_{x_i} f(x-y) \ dy \\
    \Rightarrow \quad D^\alpha u(x) &= \int_{\mathbb{R}^d} \Phi(y) D_x^\alpha f(x-y) \ dy \quad \text{for all } |\alpha| \le 2
  \end{align*}
  \(D^\alpha u(x)\)  is continuous, thus \(u \in C^2(\mathbb{R}^d)\).
  Now we check if this solves the Poisson-Equation:
  \begin{align*}
    - \Delta u(x) 
    &= \int_{\mathbb{R}^d} \Phi(y) (-\Delta_x) f(x-y) \, dy
    = \int_{\mathbb{R}^d} \Phi(y) (-\Delta_y) f(x-y) \, dy \\
    &= \int_{\mathbb{R}^d \setminus B(0, \epsilon)} \Phi(y) (-\Delta_x) f(x-y) \, dy + \int_{B(0, \epsilon)} \Phi(y) (-\Delta_x) f(x-y) \, dy \quad (\epsilon > 0 \text{ small})
  \end{align*}
  Now we come to the main part. We apply integration by parts (\ref{green-identities}):
  \begin{align*}
    &\int_{\mathbb{R}^d \setminus B(0, \epsilon)} \Phi(y)(- \Delta_y) f(x-y) \, dy \\
    &\quad = \int_{\mathbb{R}^d \setminus B(0, \epsilon)} (\nabla_y \Phi(y)) \cdot \nabla_y f(x-y) \, dy - \int_{\partial B(0, \epsilon)} \Phi(y) \cdot  \frac{\partial f}{\partial \vec{n}}(x-y) \, dS(y) \\
    &\quad = \int_{\mathbb{R}^d \setminus B(0, \epsilon)} \underbrace{(-\Delta_y \Phi(y))}_{=0} f(x-y) \, dy \\ &\qquad + \int_{\partial B(0, \epsilon)} \frac{\partial \Phi}{\partial \vec{n}}(y) f(x-y) \, dS(y) - \int_{\partial B(0, \epsilon)} \Phi(y) \frac{\partial f}{\partial \vec{n}}(x-y) \, dS(y)
  \end{align*}

  We have that \(\nabla_y \Phi(y) = -\frac{1}{d |B_1|} \frac{y}{|y|^d}\) and \( \vec{n} = \frac{y}{|y|} \text{ in } \partial B(0, \epsilon)\). This leads to
    \begin{align*}
      \frac{\partial \Phi}{\partial \vec{n}} &= \frac{1}{d |B_1|} \frac{1}{|y|^{d-1}} = \frac{1}{d |B_1| \epsilon^{d-1}} \quad \text{ for } y \in \partial B(0, \epsilon)
    \end{align*}

    Hence:
    \begin{align*}
      \int_{\partial B(0, \epsilon)} \frac{\partial \Phi}{\partial \vec{n}}(y) f(x-y) \ dS(y) 
      &= \frac{1}{d |B_1| \epsilon^{d-1}} \int_{\partial B(0, \epsilon)} f(x-y) \ dS(y) \\
      = \fint_{\partial B(0, \epsilon)} f(x-y) \ dS(y)
      &= \fint_{\partial B(x, \epsilon)} f(y) \ dS(y) 
      \xrightarrow{\epsilon \to 0} f(x)
    \end{align*}

      \begin{samepage}
        We have to regard the following error terms:
        \begin{itemize}
          \item \( 
              \begin{aligned}[t]
                \left| \int_{B(0, \epsilon)} \Phi(y) (- \Delta_y) f(x-y) \ dy\right| 
                &\le \int_{B(0, \epsilon)}|\Phi(y)| \underbrace{|-\Delta_y f(x-y)|}_{\le \|\Delta f\|_{L^\infty} \mathbb{1}(|y| \le R)} \ dy \\
                &\le \| \Delta f\|_{L^\infty} \int_{\mathbb{R}^d} \underbrace{|\Phi(y)| \mathbb{1}(|y| \le R)}_{L^1(\mathbb{R}^d)} \mathbb{1}(|y| \le \epsilon) 
                \xrightarrow{\epsilon \to 0} 0
              \end{aligned}
            \)
          Where \(R > 0\) depends on \(x\) and the support of \(f\) but is independent of \(y\).
        \item \( 
            \begin{aligned}[t]
              \left|\int_{\partial B(0, \epsilon)} \Phi(y) \frac{\partial f}{\partial \vec{n}}(x-y) \ dS(y)\right|
              &\le \|\nabla f\|_{L^\infty} \int_{\partial B(0, \epsilon)} |\Phi(y)| \ dy \\
              &\le \begin{cases}
                const \cdot \epsilon | \log \epsilon| \to 0, & d = 2 \\
                const \cdot \epsilon \to 0, & d \ge 3
              \end{cases}
            \end{aligned}
          \)
        \end{itemize}
      \end{samepage}
      Conclusion: \(-\Delta u(x) = f(x)\) for all \(x \in \mathbb{R}^d\) proved that \(u = \Phi \star f\) and \(f \in C_c^2(\mathbb{R}^d)\).
  \end{proof}

  Thus, if \(f \in C_c^2(\mathbb{R})\), then \(u = \Phi \star f\) satisfies \(u \in C^2(\mathbb{R}^2)\) and \(-\Delta u(x) = f(x)\) for all \(x \in \mathbb{R}^d\).


\begin{rem}
  The result holds for a much bigger class of functions \(f\). For example if \(f \in C_c^1(\mathbb{R})\) we can easily extend the previous proof:
  \begin{align*}
    \partial_{x_i} u = \int_{\mathbb{R}^d} \Phi(y) \partial_{x_i} f(x-y) \, dy \in C(\mathbb{R}^d) \Rightarrow u \in C^1(\mathbb{R}^d)
  \end{align*}
  Consequently: 
  \begin{align*}
    \partial_{x_i} \partial_{x_j} u 
    &= \partial_{x_i} \int_{\mathbb{R}^d} \Phi(y) \partial_{x_j} f(x-y) \, dy
    = \int_{\mathbb{R}^d} \partial_{x_i} \Phi(y) \partial_{x_j} f(x-y) \, dy \in C(\mathbb{R}^d)
  \end{align*}
  So we have \(u \in C^2(\mathbb{R}^d)\). Now we can compute
  \begin{align*}
    \Delta u = \sum_{i=1}^d \int_{\mathbb{R}^d} \partial_{x_i} \Phi(y) \partial_{x_i} f(x-y) \, dy \overset{(IBP)}{=} f(x).
  \end{align*}
\end{rem}

\begin{ex}
  Extend this to more general functions!
\end{ex}

\section{Equations in general domains}
\begin{thm}(Mean Value Theorem for Harmonic Functions)
  \label{mean-value-theorem} Let \(\Omega \subseteq \mathbb{R}\) be open, let \( u \in C^2(\Omega)\) and \(\Delta u = 0\) in \(\Omega\). Then
  \begin{align*}
    u(x) 
    &= \fint_{B(x, r)} u
    = \fint_{\partial B(x, r)} u \quad \text{for all } x \in \Omega, B(x,r) \subseteq \Omega
  \end{align*}
\end{thm}

\begin{ex}
  In 1D: \(\Delta u = 0 \Leftrightarrow u'' = 0 \Leftrightarrow u(x) = ax + b\) (Linear Equation)
\end{ex}

\begin{proof} (Of theorem \ref{mean-value-theorem})
  Consider all \(r > 0\) s.t. \(B(x,r) \subseteq \Omega\),
  \begin{align*}
    f(r) &= \fint_{\partial B(x,r)} u
  \end{align*}
  We need to prove that \(f(r)\) is independent of \(r\). When it is done, then we immediately obtain
  \begin{align*}
    f(r) = \lim_{t \to 0} f(t) = u(x)
  \end{align*}
  as \(u\) is continuous. To prove that, consider
  \begin{align*}
    f'(r) 
    &= \frac{d}{dr} \left(\fint_{\partial B(0, r)} u(x+y) \, dS(y) \right) \\
    &= \frac{d}{dr} \left(\fint_{\partial B(0, 1)} u(x + rz) \, dS(z) \right) \\
    \text{(dom. convergence)} \quad & = \fint_{\partial B(0, 1)} \frac{d}{dr} [u(x + rz)] \, dS(z) \\
    &= \fint_{\partial B(0, 1)} \nabla u(x + rz) z \, dS(z) \\
    &= \fint_{\partial B(x, r)} \nabla u(y) \frac{y-x}{r} \, dS(y) \\
    &= \frac{1}{|B(x, r)|_{\mathbb{R}^d}} \int_{\partial B(x, r)} \nabla \cdot u(y) \cdot \vec{n_y} \, dS(y) \\
    \text{(Gauss-Green \ref{gauss-green})} \quad &= \frac{1}{|B(x, r)|_{\mathbb{R}^d}} \int_{B(x, r)} \underbrace{(\Delta u)(y)}_{= 0} \, dy = 0 \qedhere
  \end{align*}
\end{proof}

\begin{rem}
  Recall the polar decomposition. Let \(x \in \mathbb{R}^d, x = (r,w), r = |x| > 0, \omega \in S^{d-1}\), then
  \begin{align*}
    \int_{\mathbb{R}^d} g(y) \, dy = \int_0^r \left(\int_{B(0, r)} g(y) \, dS(y) \right) dr
  \end{align*}
\end{rem}

We already proved that \( u(x) = \fint_{\partial B(x,r)} u \, dy \) if \(B(x,r) \subseteq \Omega\). Now we have 
\begin{align*}
  \int_{B(x, r)} u(y) \, dy 
  &= \int_{B(0, r)} u(x+y) \, dy \\
  \text{(Pol. decomposition)} \quad &= \int_0^r \left(\int_{\partial B(0, r)} u(x+y) \, dS(y)\right) ds \\
  &= \int_0^r \left(\int_{\partial B(x, s)} u(y) \, dS(y) \right) ds \\
  &= \int_0^r \left(|\partial B(x, s)| u(x) \right) ds
  = |B(x,r)| u(x)
\end{align*}
This implies
\begin{align*}
  \fint_{B(x,r)} u(y) \, dy = u(x)
  \quad \text{for any \(B(x,r) \subseteq \Omega\).}
\end{align*}

\begin{rem}
  The reverse direction is also correct, namely if \(u \in C^2(\Omega)\) and
  \begin{align*}
    u(x) 
    &= \fint_{B(x, r)} u
    = \fint_{\partial B(x,r)} u
    \quad \text{for all } B(x,r) \subseteq \Omega
  \end{align*}
  Then \(u\) is harmonic, i.e. \(\Delta u = 0\) in \(\Omega\). (The proof is exactly like before)
\end{rem}

\begin{thm} (Maximum Principle)
  Let \(\Omega \subseteq \mathbb{R}^d\) be open, let \(u \in C^2(\Omega) \cap C(\bar \Omega)\), \(\Delta u = 0\) in \(\Omega\). Then
  \begin{enumerate}
    \item \(\sup_{x \in \bar \Omega} u(x) = \sup_{x \in \partial \Omega} u(x)\)
    \item Assume that \(\Omega\) is connected. Then if there is a \(x_0 \in \Omega\) s.t. \( u(x_0) = \sup_{x \in \bar \Omega} u(x)\), then \( u \equiv const\) in \(\Omega\).
  \end{enumerate}
\end{thm}


\end{document}